Proofs/Memory_ExtraLemmas.thy
@@ -1,0 +1,197 @@
+theory Memory_ExtraLemmas
+  imports
+    "../AutoCorres/Impl"
+    "../lib/ExtraLemmas"
+    "~/Isabelle2016-1/src/HOL/Library/LaTeXsugar"
+    
+begin
+
+lemma unat_add_le: "unat (a + b) \<le> unat (a::('a::len word)) + unat b "
+  by unat_arith
+
+lemma eight_eq_eight : "unat (8::32 word) = 8" by simp
+
+lemma intvl_no_overflow_lower_bound:
+  "(a :: ('a::{len}) word) \<in> {x ..+  sz} \<Longrightarrow> unat x + sz \<le> 2 ^ LENGTH('a) \<Longrightarrow> a \<ge> x"
+  apply unat_arith unfolding intvl_def  apply unat_arith
+  apply auto 
+  apply (subgoal_tac "unat (of_nat k) = k")
+   apply (smt add.commute add_leD1 add_less_mono1 order_less_le_trans unat_of_nat unat_of_nat_eq word_nchotomy)
+  by (smt add.commute add.left_neutral add_diff_cancel_right' add_leD1 add_lessD1 diff_add_inverse 
+      diff_diff_cancel diff_le_self le_Suc_ex less_diff_conv less_irrefl_nat less_or_eq_imp_le 
+      linorder_not_less nat_add_left_cancel_less nat_less_le not_add_less1 order_less_le_trans unat_of_nat_eq)
+    
+lemma intvl_upper_bound: "a \<in> {x ..+ sz} \<Longrightarrow> 
+  unat a < unat x + sz"
+  unfolding intvl_def
+  apply unat_arith
+  apply (auto simp add: unat_of_nat) 
+  using mod_less by blast
+    
+lemma zero_not_in_intvl_lower_bound:
+  "(a::('a::len) word) \<in> {x ..+ sz} \<Longrightarrow> 0 \<notin> {x ..+  sz}  \<Longrightarrow> a \<ge>  x "
+  apply (drule zero_not_in_intvl_no_overflow)
+  by (rule intvl_no_overflow_lower_bound)
+
+lemma split_goal:"(P \<longrightarrow> Q) \<Longrightarrow> (\<not>P \<longrightarrow> Q) \<Longrightarrow> Q" 
+  by auto
+
+lemma word_div_mult_lower_bound: 
+  assumes "unat x + unat y < 2 ^ 32"
+    and "y \<noteq> 0"   
+  shows "((x:: word32) div ( y :: word32)) * y + y \<ge> x"
+proof -
+  have "unat ((x div y) * y) = unat (x div y) * unat y"
+    apply unat_arith
+    apply auto
+    by (metis (no_types, hide_lams) Word_Miscellaneous.dtle le_unat_uoi unat_div word_arith_nat_mult)
+  have "unat ((x div y) * y) = (unat x div unat y) * unat y"
+    apply unat_arith
+    apply auto
+    by (simp add: \<open>unat (x div y * y) = unat (x div y) * unat y\<close> unat_div)
+  have "unat x div unat y * unat y + unat x mod unat y = unat x"
+    by simp
+  show ?thesis
+    using `unat x + unat y < 2 ^ 32` `y \<noteq> 0` 
+      `unat ((x div y) * y) = (unat x div unat y) * unat y`
+  apply unat_arith
+  apply auto  
+   apply unat_arith
+     apply auto
+    apply (subgoal_tac "unat x div unat y * unat y + unat x mod unat y = unat x")
+     apply (metis mod_le_divisor nat_add_left_cancel_le)
+     apply simp
+    using `unat x div unat y * unat y + unat x mod unat y = unat x`
+      by arith
+qed
+
+lemma scast_NOT_simp: "(scast (~~(flag :: 32 signed word)) :: word32) = ~~ ((scast flag)::word32)"
+  unfolding word_not_def
+  apply (subst scast_down_wi)
+   defer
+   apply (subst uint_scast)
+   apply (rule refl)
+  apply (subst is_down)
+  by simp  
+
+    
+(* Unused *)    
+lemma c_guard_l1:
+  assumes "c_guard (a::('a::mem_type) ptr)"
+    "\<not> c_guard (a +\<^sub>p 1)"
+    "b > a" 
+    "b \<ge> a +\<^sub>p 1"
+  shows "\<not> c_null_guard b" 
+proof -
+  have "\<not> c_null_guard ( a +\<^sub>p 1)" using `c_guard a` `\<not> c_guard (a +\<^sub>p 1)`
+    unfolding c_guard_def apply auto    
+    apply(frule ptr_aligned_plus[where i = 1]) by auto
+  hence "0 \<in> ptr_span (a +\<^sub>p 1)" unfolding c_null_guard_def by auto
+  have "0 \<in> ptr_span b" using `b \<ge> a +\<^sub>p 1` using `0 \<in> ptr_span (a +\<^sub>p 1)` unfolding intvl_def
+  proof simp
+    assume "a +\<^sub>p 1 \<le> b"
+      and "\<exists>k. ptr_val (a +\<^sub>p 1) + of_nat k = 0 \<and> k < size_of TYPE('a)"
+    then obtain k where k:"ptr_val (a +\<^sub>p 1) + of_nat k = 0 \<and> k < size_of TYPE('a)" by auto
+    hence "ptr_val (a +\<^sub>p 1) + of_nat k = 0" by auto
+    {
+      assume "((of_nat k)::32 word) \<noteq> 0"
+      have "ptr_val b \<ge> ptr_val (a +\<^sub>p 1)" using `b \<ge> a +\<^sub>p 1`  by (simp add: ptr_le_def ptr_le_def')
+      hence 1:"ptr_val b - ptr_val (a +\<^sub>p 1) \<le> of_nat k" 
+        using `ptr_val (a +\<^sub>p 1) + of_nat k = 0`
+        apply unat_arith apply auto
+        using `of_nat k \<noteq> 0` 
+        apply (subgoal_tac "unat ((of_nat k)::32 word) = 0 \<Longrightarrow> ((of_nat k)::32 word) = 0")
+         apply auto[1]
+        apply (subst (asm) (3) unat_eq_0)  by auto
+          
+      let ?k2' = "of_nat k - ( ptr_val b - ptr_val (a +\<^sub>p 1))"
+      have "ptr_val b + ?k2' = of_nat k + ptr_val (a +\<^sub>p 1)" by simp
+      hence "ptr_val b + ?k2' = 0" using k by (simp add: add.commute)
+      hence 2:"ptr_val b + of_nat (unat ?k2') = 0" by simp
+          
+      let ?of_nat_k = "((of_nat k):: 32 word)"
+      have "?k2' \<le> ?of_nat_k" using 1  word_sub_le by auto
+      hence "unat ?k2' \<le> unat ?of_nat_k" by (simp add: word_le_nat_alt) 
+      moreover have "unat ?of_nat_k \<le> k" by (metis le_cases le_unat_uoi) 
+      moreover  have "k < size_of TYPE('a)" using k by simp
+      ultimately have "(unat ?k2') < size_of TYPE('a)" by simp
+      hence "ptr_val b + of_nat (unat ?k2') = 0 \<and> (unat ?k2') < size_of TYPE('a)" using 2 by simp
+      hence "\<exists>k::nat. ptr_val b + of_nat k = (0::32 word) \<and> k < size_of TYPE('a)" by (frule exI)
+    }
+    moreover{  
+      assume k_eq_0:"((of_nat k)::32 word) = 0" 
+      let ?k2' = "of_nat (size_of TYPE('a)) - ( ptr_val b - ptr_val a)"
+      have "ptr_val b > ptr_val a" using `b>a` 
+        by (simp add: ptr_less_def ptr_less_def')
+      hence "unat (ptr_val b) > unat (ptr_val a)" using unat_mono by auto
+      from k_eq_0 have "ptr_val (a +\<^sub>p 1)= 0" using k by unat_arith
+      hence 1:"ptr_val a + of_nat (size_of TYPE('a)) = 0" unfolding ptr_add_def by simp
+      hence 2: "ptr_val b - ptr_val a < of_nat (size_of TYPE('a))" 
+        using k_eq_0
+        apply unat_arith (* SLOW! *) apply auto
+         apply (subgoal_tac "unat (ptr_val a) \<noteq> (0::nat)")
+          apply auto[1]
+        using `c_guard a` 
+         apply (metis len_of_addr_card max_size mem_type_simps(3) neq0_conv unat_of_nat_len)
+        using `unat (ptr_val b) > unat (ptr_val a)` by simp
+      hence "ptr_val b + ?k2' = 0" using 1  by (simp add: add.commute)
+      hence 3:"ptr_val b + of_nat (unat ?k2') = 0" by simp
+      have "ptr_val b - ptr_val a > 0" using `ptr_val b > ptr_val a` 
+        using word_neq_0_conv by fastforce 
+      with 2 have "?k2' < of_nat (size_of TYPE('a))"  by unat_arith (* VERY SLOW! *)
+      hence "unat ?k2' < size_of TYPE('a)" using unat_less_helper by auto
+      with 3 have "ptr_val b + of_nat (unat ?k2') = 0 \<and> unat ?k2' < size_of TYPE('a)" by auto
+      hence "\<exists>k::nat. ptr_val b + of_nat k = (0::32 word) \<and> k < size_of TYPE('a)" by (frule exI)  
+    }
+    ultimately show "\<exists>k::nat. ptr_val b + of_nat k = (0::32 word) \<and> k < size_of TYPE('a)"
+      by auto
+  qed 
+  thus "\<not> c_null_guard b" unfolding c_null_guard_def by auto
+qed
+   
+lemma unat_add_lem_3:
+  "unat (a::'a::len word) + unat b + unat c < 2 ^ LENGTH('a) =
+    (unat (a + b + c) = unat a + unat b + unat c)"
+  using unat_add_lem
+  by (metis add_lessD1 unat_lt2p) 
+    
+lemma unat_addition_less_pres:"unat (a::'a::len word) + unat b < unat c \<Longrightarrow> a + b < c"
+  by unat_arith
+    
+lemma unat_addition_le_pres:"unat (a::'a::len word) + unat b \<le> unat c \<Longrightarrow> a + b \<le> c"
+  by unat_arith
+    
+lemma shiftr3_upper_bound:"(x :: 32 word) >> 3 \<le> 0x1FFFFFFF"
+  apply (simp add:shiftr3_is_div_8)
+  apply unat_arith
+  by auto
+  
+lemma intvl_no_overflow2:
+  assumes asm: "unat (a::'a::len word) + b \<le> 2 ^ LENGTH('a)"
+  shows "(x \<in> {a..+b}) = (a \<le> x \<and> unat x < unat a + b)"
+proof -
+  {
+    assume "x \<in> {a ..+ b}"
+    with intvl_no_overflow_lower_bound intvl_upper_bound asm
+    have "(a \<le> x \<and> unat x < unat a + b)" by blast    
+  }moreover
+  {
+    assume "(a \<le> x \<and> unat x < unat a + b)"
+    thm intvlI   
+    have "a + of_nat (unat x - unat a) \<in> {a ..+ b}"
+      apply (rule intvlI)
+      using `(a \<le> x \<and> unat x < unat a + b)` asm
+      by unat_arith
+    moreover have "a + of_nat (unat x - unat a) = x" 
+      using `(a \<le> x \<and> unat x < unat a + b)` asm
+      apply unat_arith
+      apply (subgoal_tac "unat (x - a) = unat x - unat a")
+       apply auto
+      by unat_arith
+    ultimately have "x \<in> {a ..+ b}" by argo
+  }
+  ultimately show ?thesis by fast  
+qed
+
+    
+end
